

1 Definition

A *field* \mathbf{F} is a set containing at least two distinct elements called 0 and 1, along with operations of addition and multiplication satisfying all the properties listed below.

1. Commutativity

$$\alpha + \beta = \beta + \alpha \text{ and } \alpha\beta = \beta\alpha, \text{ for all } \alpha, \beta \in \mathbf{F}.$$

2. Associativity

$$(\alpha + \beta) + \lambda = \alpha + (\beta + \lambda) \text{ and } (\alpha\beta)\lambda = \alpha(\beta\lambda), \text{ for all } \alpha, \beta, \lambda \in \mathbf{F}.$$

3. Identities

$$\lambda + 0 = \lambda \text{ and } 1\lambda = \lambda, \text{ for all } \lambda \in \mathbf{F}.$$

4. Additive Inverse

$$\text{For every } \alpha \in \mathbf{F}, \text{ there exists a unique } \beta \in \mathbf{F} \text{ such that } \alpha + \beta = 0.$$

5. Multiplicative Inverse

$$\text{For every } \alpha \in \mathbf{F} \text{ with } \alpha \neq 0, \text{ there exists a unique } \beta \in \mathbf{F} \text{ such that } \alpha\beta = 1.$$

6. Distributive Property

$$\lambda(\alpha + \beta) = \lambda\alpha + \lambda\beta, \text{ for all } \lambda, \alpha, \beta \in \mathbf{F}.$$

Note

In linear algebra we rarely deal with fields other than \mathbf{R} and \mathbf{C} , but other fields do exist such as the set of rational numbers along with the usual operations of addition and multiplication, and the set $\{0, 1\}$ with the usual operations of addition and multiplication except that $1 + 1$ is defined to equal 0.

2 Exercise

Prove that the set of *complex numbers* with the following operations of addition and multiplication is a field. For the sake of simplicity, we can trivially say that \mathbf{R} is a field, and safely use all calculation techniques from \mathbf{R} .

2.1 Definition

- A complex number is an ordered pair (a, b) , where $a, b \in \mathbf{R}$, written as $a + bi$.
- The set of all complex numbers is denoted by \mathbf{C} :

$$\mathbf{C} = \{a + bi \mid a, b \in \mathbf{R}\}.$$

- Addition and multiplication on \mathbf{C} are defined by

$$(a + bi) + (c + di) = (a + c) + (b + d)i, \quad (1)$$

$$(a + bi)(c + di) = (ac - bd) + (ad + bc)i; \quad (2)$$

with $a, b, c, d \in \mathbf{R}$.

2.2 Proof

1. Commutativity

For all $\alpha, \beta \in \mathbf{C}$, we can write $\alpha = a + bi$ and $\beta = c + di$ with some $a, b, c, d \in \mathbf{R}$, then

$$\begin{aligned} \alpha + \beta &= (a + bi) + (c + di) \\ &= (a + c) + (b + d)i && \text{by (1)} \end{aligned}$$

$$\begin{aligned} \beta + \alpha &= (c + di) + (a + bi) \\ &= (c + a) + (d + b)i && \text{by (1)} \\ &= \alpha + \beta && \text{by comm. of } \mathbf{R} \end{aligned}$$

$$\begin{aligned} \alpha\beta &= (a + bi)(c + di) \\ &= (ac - bd) + (ad + bc)i && \text{by (2)} \end{aligned}$$

$$\begin{aligned} \beta\alpha &= (c + di)(a + bi) \\ &= (ca - db) + (da + cb)i && \text{by (2)} \\ &= \alpha\beta && \text{by comm. of } \mathbf{R} \end{aligned}$$

2. Associativity

For all $\alpha, \beta, \lambda \in \mathbf{C}$, write $\alpha = a + bi$, $\beta = c + di$, $\lambda = e + fi$ with some $a, b, c, d, e, f \in \mathbf{R}$, then

$$\begin{aligned}
 (\alpha + \beta) + \lambda &= [(a + bi) + (c + di)] + (e + fi) \\
 &= [(a + c) + (b + d)i] + (e + fi) && \text{by (1)} \\
 &= [(a + c) + e] + [(b + d) + f]i && \text{by (1)} \\
 \alpha + (\beta + \lambda) &= (a + bi) + [(c + di) + (e + fi)] \\
 &= (a + bi) + [(c + e) + (d + f)i] && \text{by (1)} \\
 &= [a + (c + e)] + [b + (d + f)]i && \text{by (1)} \\
 &= (\alpha + \beta) + \lambda && \text{by asso. of } \mathbf{R}
 \end{aligned}$$

$$\begin{aligned}
 (\alpha\beta)\lambda &= [(a + bi)(c + di)](e + fi) \\
 &= [(ac - bd) + (ad + bc)i](e + fi) && \text{by (2)} \\
 &= [(ac - bd)e - (ad + bc)f] + [(ac - bd)f + (ad + bc)e]i && \text{by (2)} \\
 &= (ace - bde - adf - bcf) + (acf - bdf + ade + bce)i && \text{by dist. of } \mathbf{R} \\
 \alpha(\beta\lambda) &= (a + bi)[(c + di)(e + fi)] \\
 &= (a + bi)[(ce - df) + (cf + de)i] && \text{by (2)} \\
 &= [a(ce - df) - b(cf + de)] + [a(cf + de) + b(ce - df)]i && \text{by (2)} \\
 &= (ace - bde - adf - bcf) + (acf - bdf + ade + bce)i && \text{by dist. of } \mathbf{R} \\
 &= (\alpha\beta)\lambda && \text{by comm. of } \mathbf{R}
 \end{aligned}$$

3. Identities

For all $\lambda \in \mathbf{C}$, write $\lambda = a + bi$ for some $a, b \in \mathbf{R}$, then

$$\begin{aligned}
 \lambda + 0 &= (a + bi) + (0 + 0i) \\
 &= (a + 0) + (b + 0)i && \text{by (1)} \\
 &= a + bi && \text{by iden. of } \mathbf{R} \\
 &= \lambda
 \end{aligned}$$

$$\begin{aligned}
 1\lambda &= (1 + 0i)(a + bi) \\
 &= (1a + 0b) + (1b + 0a)i && \text{by (2)} \\
 &= a + bi && \text{by iden. and mul. of } \mathbf{R} \\
 &= \lambda
 \end{aligned}$$

4. Additive Inverse

For every $\alpha \in \mathbf{C}$, write $\alpha = a + bi$ for some $a, b \in \mathbf{R}$, then we can find a unique $\beta = c + di \in \mathbf{C}$ such that $\alpha + \beta = 0$ by the following manner:

$$\begin{aligned}\alpha + \beta &= (a + bi) + (c + di) \\ &= (a + c) + (b + d)i && \text{by (1)} \\ &= 0 + 0i && \text{by assumption} \\ \Rightarrow (c, d) &= (-a, -b) && \text{by add.inv. of } \mathbf{R}\end{aligned}$$

Thus β is the unique additive inverse of α .

5. Multiplicative Inverse

For every $\alpha \in \mathbf{C}$, write $\alpha = a + bi$ for some $a, b \in \mathbf{R}$ with $a \neq 0$ and $b \neq 0$, then we can find a unique $\beta = c + di \in \mathbf{C}$ such that $\alpha\beta = 1$ by the following manner:

$$\begin{aligned}\alpha\beta &= (a + bi)(c + di) \\ &= (ac - bd) + (ad + bc)i && \text{by (2)} \\ &= 1 + 0i && \text{by assumption}\end{aligned}$$

That is, $ac - bd = 1$ and $ad + bc = 0$. By solving these two equations for c and d , we have

$$(c, d) = \left(\frac{a}{a^2 + b^2}, \frac{-b}{a^2 + b^2} \right),$$

thus β is the unique multiplicative inverse of α .

6. Distributive Property

For all $\alpha, \beta, \lambda \in \mathbf{C}$, write $\alpha = a + bi$, $\beta = c + di$, $\lambda = e + fi$ with some $a, b, c, d, e, f \in \mathbf{R}$, then

$$\begin{aligned}\lambda(\alpha + \beta) &= (e + fi)[(a + bi) + (c + di)] \\ &= (e + fi)[(a + c) + (b + d)i] && \text{by (1)} \\ &= [e(a + c) - f(b + d)] + [e(b + d) + f(a + c)]i && \text{by (2)} \\ &= (ea + ec - fb - fd) + (eb + ed + fa + fc)i && \text{by dist. of } \mathbf{R}\end{aligned}$$

$$\begin{aligned}\lambda\alpha + \lambda\beta &= [(e + fi)(a + bi)] + [(e + fi)(c + di)] \\ &= [(ea - fb) + (eb + fa)i] + [(ec - fd) + (ed + fc)i] && \text{by (2)} \\ &= (ea - fb + ec - fd) + (eb + fa + ed + fc)i && \text{by (1)} \\ &= \lambda(\alpha + \beta) && \text{by comm. of } \mathbf{R}\end{aligned}$$